Add metadata field to operations and trees

Move.thy
@@ -4,41 +4,50 @@ begin
 
 section \<open>Definitions\<close>
 
-datatype ('time, 'node) operation
-  = Move (move_time: 'time) (move_parent: 'node) (move_child: 'node)
+datatype ('t, 'n, 'm) operation
+  = Move (move_time: 't)
+         (move_parent: 'n)
+         (move_meta: 'm)
+         (move_child: 'n)
 
-datatype ('time, 'node) log_op
-  = LogMove (log_time: 'time) (old_parent: \<open>'node option\<close>) (new_parent: 'node) (log_child: 'node)
+datatype ('t, 'n, 'm) log_op
+  = LogMove (log_time: 't)
+            (old_parent: \<open>('n \<times> 'm) option\<close>)
+            (new_parent: 'n)
+            (log_meta: 'm)
+            (log_child: 'n)
 
-type_synonym ('t, 'n) state = \<open>('t, 'n) log_op list \<times> ('n \<times> 'n) set\<close>
+type_synonym ('t, 'n, 'm) state = \<open>('t, 'n, 'm) log_op list \<times> ('n \<times> 'm \<times> 'n) set\<close>
 
-definition get_parent :: \<open>('n \<times> 'n) set \<Rightarrow> 'n \<Rightarrow> 'n option\<close> where
+definition get_parent :: \<open>('n \<times> 'm \<times> 'n) set \<Rightarrow> 'n \<Rightarrow> ('n \<times> 'm) option\<close> where
   \<open>get_parent tree child \<equiv>
-     if \<exists>!parent. (parent, child) \<in> tree then
-       Some (THE parent. (parent, child) \<in> tree)
+     if \<exists>!parent. \<exists>!meta. (parent, meta, child) \<in> tree then
+       Some (THE (parent, meta). (parent, meta, child) \<in> tree)
      else None\<close>
 
-inductive ancestor :: \<open>('n \<times> 'n) set \<Rightarrow> 'n \<Rightarrow> 'n \<Rightarrow> bool\<close> where
-  \<open>\<lbrakk>(parent, child) \<in> tree\<rbrakk> \<Longrightarrow> ancestor tree parent child\<close> |
-  \<open>\<lbrakk>(parent, child) \<in> tree; ancestor tree anc parent\<rbrakk> \<Longrightarrow> ancestor tree anc child\<close>
+inductive ancestor :: \<open>('n \<times> 'm \<times> 'n) set \<Rightarrow> 'n \<Rightarrow> 'n \<Rightarrow> bool\<close> where
+  \<open>\<lbrakk>(parent, meta, child) \<in> tree\<rbrakk> \<Longrightarrow> ancestor tree parent child\<close> |
+  \<open>\<lbrakk>(parent, meta, child) \<in> tree; ancestor tree anc parent\<rbrakk> \<Longrightarrow> ancestor tree anc child\<close>
 
-fun do_op :: \<open>('t, 'n) operation \<times> ('n \<times> 'n) set \<Rightarrow> ('t, 'n) log_op \<times> ('n \<times> 'n) set\<close> where
-  \<open>do_op (Move t newp c, tree) =
-     (LogMove t (get_parent tree c) newp c,
+fun do_op :: \<open>('t, 'n, 'm) operation \<times> ('n \<times> 'm \<times> 'n) set \<Rightarrow>
+              ('t, 'n, 'm) log_op \<times> ('n \<times> 'm \<times> 'n) set\<close> where
+  \<open>do_op (Move t newp m c, tree) =
+     (LogMove t (get_parent tree c) newp m c,
       if ancestor tree c newp \<or> c = newp then tree
-      else {(p', c') \<in> tree. c' \<noteq> c} \<union> {(newp, c)})\<close>
+      else {(p', m', c') \<in> tree. c' \<noteq> c} \<union> {(newp, m, c)})\<close>
 
-fun undo_op :: \<open>('t, 'n) log_op \<times> ('n \<times> 'n) set \<Rightarrow> ('n \<times> 'n) set\<close> where
-  \<open>undo_op (LogMove t None newp c, tree) = {(p', c') \<in> tree. c' \<noteq> c}\<close> |
-  \<open>undo_op (LogMove t (Some oldp) newp c, tree) =
-     {(p', c') \<in> tree. c' \<noteq> c} \<union> {(oldp, c)}\<close>
+fun undo_op :: \<open>('t, 'n, 'm) log_op \<times> ('n \<times> 'm \<times> 'n) set \<Rightarrow> ('n \<times> 'm \<times> 'n) set\<close> where
+  \<open>undo_op (LogMove t None newp m c, tree) = {(p', m', c') \<in> tree. c' \<noteq> c}\<close> |
+  \<open>undo_op (LogMove t (Some (oldp, oldm)) newp m c, tree) =
+     {(p', m', c') \<in> tree. c' \<noteq> c} \<union> {(oldp, oldm, c)}\<close>
 
-fun redo_op :: \<open>('t, 'n) log_op \<Rightarrow> ('t, 'n) state \<Rightarrow> ('t, 'n) state\<close> where
-  \<open>redo_op (LogMove t _ p c) (ops, tree) =
-     (let (op2, tree2) = do_op (Move t p c, tree)
+fun redo_op :: \<open>('t, 'n, 'm) log_op \<Rightarrow> ('t, 'n, 'm) state \<Rightarrow> ('t, 'n, 'm) state\<close> where
+  \<open>redo_op (LogMove t _ p m c) (ops, tree) =
+     (let (op2, tree2) = do_op (Move t p m c, tree)
       in (op2 # ops, tree2))\<close>
 
-fun interp_op :: \<open>('t::{linorder}, 'n) operation \<Rightarrow> ('t, 'n) state \<Rightarrow> ('t, 'n) state\<close> where
+fun interp_op :: \<open>('t::{linorder}, 'n, 'm) operation \<Rightarrow>
+                  ('t, 'n, 'm) state \<Rightarrow> ('t, 'n, 'm) state\<close> where
   \<open>interp_op op1 ([], tree1) =
      (let (op2, tree2) = do_op (op1, tree1)
       in ([op2], tree2))\<close> |
@@ -47,148 +56,229 @@ fun interp_op :: \<open>('t::{linorder}, 'n) operation \<Rightarrow> ('t, 'n) st
       then redo_op logop (interp_op op1 (ops, undo_op (logop, tree1)))
       else let (op2, tree2) = do_op (op1, tree1) in (op2 # logop # ops, tree2))\<close>
 
-definition interp_ops :: \<open>('t::{linorder}, 'n) operation list \<Rightarrow> ('t, 'n) log_op list \<times> ('n \<times> 'n) set\<close> where
+definition interp_ops :: \<open>('t::{linorder}, 'n, 'm) operation list \<Rightarrow> ('t, 'n, 'm) state\<close> where
   \<open>interp_ops ops \<equiv> foldl (\<lambda>state oper. interp_op oper state) ([], {}) ops\<close>
+
+definition unique_parent :: \<open>('n \<times> 'm \<times> 'n) set \<Rightarrow> bool\<close> where
+  \<open>unique_parent tree \<equiv> (\<forall>p1 p2 m1 m2 c. (p1, m1, c) \<in> tree \<and> (p2, m2, c) \<in> tree \<longrightarrow> p1 = p2 \<and> m1 = m2)\<close>
 
 
 section \<open>undo-op is the inverse of do-op\<close>
 
 lemma get_parent_None:
-  assumes \<open>\<nexists>p. (p, c) \<in> tree\<close>
+  assumes \<open>\<nexists>p m. (p, m, c) \<in> tree\<close>
   shows \<open>get_parent tree c = None\<close>
   by (meson assms get_parent_def)
 
-lemma get_parent_empty [simp]:
-  shows \<open>get_parent {} p = None\<close>
-  using get_parent_None by force
-
 lemma get_parent_Some:
-  assumes \<open>(p, c) \<in> tree\<close>
-    and \<open>\<And>x. (x, c) \<in> tree \<Longrightarrow> x = p\<close>
-  shows \<open>get_parent tree c = Some p\<close>
+  assumes \<open>(p, m, c) \<in> tree\<close>
+    and \<open>\<And>p' m'. (p', m', c) \<in> tree \<Longrightarrow> p' = p \<and> m' = m\<close>
+  shows \<open>get_parent tree c = Some (p, m)\<close>
 proof -
-  have \<open>\<exists>!parent. (parent, c) \<in> tree\<close>
+  have \<open>\<exists>!parent. \<exists>!meta. (parent, meta, c) \<in> tree\<close>
     using assms by metis
-  hence \<open>(THE parent. (parent, c) \<in> tree) = p\<close>
-    using assms(2) by fastforce
-  thus \<open>get_parent tree c = Some p\<close>
+  hence \<open>(THE (parent, meta). (parent, meta, c) \<in> tree) = (p, m)\<close>
+    using assms(2) by auto
+  thus \<open>get_parent tree c = Some (p, m)\<close>
     using assms get_parent_def by metis
 qed
 
+lemma pred_equals_eq3:
+  shows \<open>(\<lambda>x y z. (x, y, z) \<in> R) = (\<lambda>x y z. (x, y, z) \<in> S) \<longleftrightarrow> R = S\<close>
+  by (simp add: set_eq_iff fun_eq_iff)
+
 lemma do_undo_op_inv:
-  assumes \<open>\<And>x. (x, c) \<in> tree \<Longrightarrow> x = oldp\<close>
-  shows \<open>undo_op (do_op (Move t p c, tree)) = tree\<close>
-proof(cases \<open>\<exists>par. (par, c) \<in> tree\<close>)
+  assumes \<open>unique_parent tree\<close>
+  shows \<open>undo_op (do_op (Move t p m c, tree)) = tree\<close>
+proof(cases \<open>\<exists>par meta. (par, meta, c) \<in> tree\<close>)
   case True
-  hence 1: \<open>(oldp, c) \<in> tree\<close>
-    using assms by blast
-  hence 2: \<open>get_parent tree c = Some oldp\<close>
-    using assms get_parent_Some by metis
-  moreover have \<open>\<And>p' c'. (p', c') \<in> tree \<Longrightarrow> (p', c') \<in> undo_op (do_op (Move t p c, tree))\<close>
-    using assms calculation by auto
-  moreover have \<open>\<And>p' c'. (p', c') \<in> undo_op (do_op (Move t p c, tree)) \<Longrightarrow> (p', c') \<in> tree\<close>
-    using 1 2 by (cases \<open>ancestor tree c p \<or> c = p\<close>, auto)
+  from this obtain oldp oldm where 1: \<open>(oldp, oldm, c) \<in> tree\<close>
+    by blast
+  hence 2: \<open>get_parent tree c = Some (oldp, oldm)\<close>
+    using assms get_parent_Some unique_parent_def by metis
+  {
+    fix p' m' c'
+    assume 3: \<open>(p', m', c') \<in> tree\<close>
+    have \<open>(p', m', c') \<in> undo_op (do_op (Move t p m c, tree))\<close>
+    proof(cases \<open>c = c'\<close>)
+      case True
+      then show ?thesis using 1 2 3 assms unique_parent_def by fastforce
+    next
+      case False
+      then show ?thesis using 2 3 by auto
+    qed
+  }
+  hence \<open>tree \<subseteq> undo_op (do_op (Move t p m c, tree))\<close>
+    by auto
+  moreover have \<open>undo_op (do_op (Move t p m c, tree)) \<subseteq> tree\<close>
+    using 1 2 by auto
   ultimately show ?thesis
-    by (meson pred_equals_eq2)
+    by blast
 next
   case no_old_parent: False
   hence \<open>get_parent tree c = None\<close>
     using assms get_parent_None by metis
-  moreover have \<open>{(p', c') \<in> tree. c' \<noteq> c} = tree\<close>
+  moreover have \<open>{(p', m', c') \<in> tree. c' \<noteq> c} = tree\<close>
     using no_old_parent by fastforce
-  moreover from this have \<open>{(p', c') \<in> (tree \<union> {(p, c)}). c' \<noteq> c} = tree\<close>
-    by auto
+  moreover from this have \<open>{(p', m', c') \<in> (tree \<union> {(p, m, c)}). c' \<noteq> c} = tree\<close>
+    by blast
   ultimately show ?thesis by simp
 qed
 
 
 section \<open>Preserving the invariant that each tree node has at most one parent\<close>
 
+lemma subset_unique_parent:
+  assumes \<open>unique_parent tree\<close>
+  shows \<open>unique_parent {(p', m', c') \<in> tree. c' \<noteq> c}\<close>
+proof -
+  {
+    fix p1 p2 m1 m2 c'
+    assume 1: \<open>(p1, m1, c') \<in> {(p', m', c') \<in> tree. c' \<noteq> c}\<close>
+       and 2: \<open>(p2, m2, c') \<in> {(p', m', c') \<in> tree. c' \<noteq> c}\<close>
+    have \<open>p1 = p2 \<and> m1 = m2\<close>
+    proof(cases \<open>c = c'\<close>)
+      case True
+      then show ?thesis using 1 2 by auto
+    next
+      case False
+      hence \<open>(p1, m1, c') \<in> tree \<and> (p2, m2, c') \<in> tree\<close>
+        using 1 2 by blast
+      then show ?thesis
+        using assms by (meson unique_parent_def)
+    qed
+  }
+  thus ?thesis by (meson unique_parent_def)
+qed
+
+lemma subset_union_unique_parent:
+  assumes \<open>unique_parent tree\<close>
+  shows \<open>unique_parent ({(p', m', c') \<in> tree. c' \<noteq> c} \<union> {(p, m, c)})\<close>
+proof -
+  {
+    fix p1 p2 m1 m2 c'
+    assume 1: \<open>(p1, m1, c') \<in> {(p', m', c') \<in> tree. c' \<noteq> c} \<union> {(p, m, c)}\<close>
+       and 2: \<open>(p2, m2, c') \<in> {(p', m', c') \<in> tree. c' \<noteq> c} \<union> {(p, m, c)}\<close>
+    have \<open>p1 = p2 \<and> m1 = m2\<close>
+    proof(cases \<open>c = c'\<close>)
+      case True
+      then show ?thesis using 1 2 by auto
+    next
+      case False
+      hence \<open>(p1, m1, c') \<in> tree \<and> (p2, m2, c') \<in> tree\<close>
+        using 1 2 by blast
+      then show ?thesis
+        using assms by (meson unique_parent_def)
+    qed
+  }
+  thus ?thesis by (meson unique_parent_def)
+qed
+
 lemma do_op_unique_parent:
-  assumes \<open>\<And>p1 p2 c. (p1, c) \<in> tree1 \<Longrightarrow> (p2, c) \<in> tree1 \<Longrightarrow> p1 = p2\<close>
-    and \<open>do_op (Move t newp c, tree1) = (log_oper, tree2)\<close>
-  shows \<open>\<And>p1 p2 c. (p1, c) \<in> tree2 \<Longrightarrow> (p2, c) \<in> tree2 \<Longrightarrow> p1 = p2\<close>
+  assumes \<open>unique_parent tree1\<close>
+    and \<open>do_op (Move t newp m c, tree1) = (log_oper, tree2)\<close>
+  shows \<open>unique_parent tree2\<close>
 proof(cases \<open>ancestor tree1 c newp \<or> c = newp\<close>)
   case True
-  then show \<open>\<And>p1 p2 c. (p1, c) \<in> tree2 \<Longrightarrow> (p2, c) \<in> tree2 \<Longrightarrow> p1 = p2\<close>
-    using assms by auto
+  hence \<open>tree1 = tree2\<close>
+    using assms(2) by auto
+  thus \<open>unique_parent tree2\<close>
+    by (metis (full_types) assms(1))
 next
   case False
-  hence \<open>tree2 = {(p', c') \<in> tree1. c' \<noteq> c} \<union> {(newp, c)}\<close>
+  hence \<open>tree2 = {(p', m', c') \<in> tree1. c' \<noteq> c} \<union> {(newp, m, c)}\<close>
     using assms(2) by auto
-  then show \<open>\<And>p1 p2 c. (p1, c) \<in> tree2 \<Longrightarrow> (p2, c) \<in> tree2 \<Longrightarrow> p1 = p2\<close>
-    using assms(1) by auto
+  then show \<open>unique_parent tree2\<close>
+    using subset_union_unique_parent assms(1) by fastforce
 qed
 
 lemma undo_op_unique_parent:
-  assumes \<open>\<And>p1 p2 c. (p1, c) \<in> tree1 \<Longrightarrow> (p2, c) \<in> tree1 \<Longrightarrow> p1 = p2\<close>
-    and \<open>undo_op (LogMove t oldp newp c, tree1) = tree2\<close>
-  shows \<open>\<And>p1 p2 c. (p1, c) \<in> tree2 \<Longrightarrow> (p2, c) \<in> tree2 \<Longrightarrow> p1 = p2\<close>
-using assms by (cases oldp, auto)
+  assumes \<open>unique_parent tree1\<close>
+    and \<open>undo_op (LogMove t oldp newp m c, tree1) = tree2\<close>
+  shows \<open>unique_parent tree2\<close>
+proof (cases oldp)
+  case None
+  hence \<open>tree2 = {(p', m', c') \<in> tree1. c' \<noteq> c}\<close>
+    using assms(2) by auto
+  then show ?thesis
+    by (simp add: assms(1) subset_unique_parent)
+next
+  case (Some old)
+  obtain oldp oldm where \<open>old = (oldp, oldm)\<close>
+    by fastforce
+  hence \<open>tree2 = {(p', m', c') \<in> tree1. c' \<noteq> c} \<union> {(oldp, oldm, c)}\<close>
+    using Some assms(2) by auto
+  then show ?thesis
+    using subset_union_unique_parent assms(1) by fastforce
+qed
 
 lemma redo_op_unique_parent:
-  assumes \<open>\<And>p1 p2 c. (p1, c) \<in> tree1 \<Longrightarrow> (p2, c) \<in> tree1 \<Longrightarrow> p1 = p2\<close>
+  assumes \<open>unique_parent tree1\<close>
     and \<open>redo_op oper (ops1, tree1) = (ops2, tree2)\<close>
-  shows \<open>\<And>p1 p2 c. (p1, c) \<in> tree2 \<Longrightarrow> (p2, c) \<in> tree2 \<Longrightarrow> p1 = p2\<close>
+  shows \<open>unique_parent tree2\<close>
 proof -
-  obtain t oldp newp c where \<open>oper = LogMove t oldp newp c\<close>
+  obtain t oldp newp m c where \<open>oper = LogMove t oldp newp m c\<close>
     using log_op.exhaust by blast
-  from this obtain move2 where \<open>(move2, tree2) = do_op (Move t newp c, tree1)\<close>
+  from this obtain move2 where \<open>(move2, tree2) = do_op (Move t newp m c, tree1)\<close>
     using assms(2) by auto
-  thus \<open>\<And>p1 p2 c. (p1, c) \<in> tree2 \<Longrightarrow> (p2, c) \<in> tree2 \<Longrightarrow> p1 = p2\<close>
+  thus \<open>unique_parent tree2\<close>
     by (metis assms(1) do_op_unique_parent)
 qed
 
-theorem interp_op_unique_parent:
-  assumes \<open>\<And>p1 p2 c. (p1, c) \<in> tree1 \<Longrightarrow> (p2, c) \<in> tree1 \<Longrightarrow> p1 = p2\<close>
+lemma interp_op_unique_parent:
+  assumes \<open>unique_parent tree1\<close>
     and \<open>interp_op oper (ops1, tree1) = (ops2, tree2)\<close>
-  shows \<open>\<And>p1 p2 c. (p1, c) \<in> tree2 \<Longrightarrow> (p2, c) \<in> tree2 \<Longrightarrow> p1 = p2\<close>
+  shows \<open>unique_parent tree2\<close>
 using assms proof(induct ops1 arbitrary: tree1 tree2 ops2)
   case Nil
   have \<open>\<And>pair. snd (case pair of (p1, p2) \<Rightarrow> ([p1], p2)) = snd pair\<close>
     by (simp add: prod.case_eq_if)
   hence \<open>\<exists>log_op. do_op (oper, tree1) = (log_op, tree2)\<close>
-    by (metis Nil.prems(4) interp_op.simps(1) old.prod.exhaust snd_conv)
-  thus \<open>\<And>p1 p2 c. (p1, c) \<in> tree2 \<Longrightarrow> (p2, c) \<in> tree2 \<Longrightarrow> p1 = p2\<close>
-    by (metis Nil.prems(3) do_op_unique_parent operation.exhaust_sel)
+    by (metis Nil.prems(2) interp_op.simps(1) prod.collapse snd_conv)
+  thus \<open>unique_parent tree2\<close>
+    by (metis Nil.prems(1) do_op_unique_parent operation.exhaust_sel)
 next
   case step: (Cons logop ops)
-  then show \<open>\<And>p1 p2 c. (p1, c) \<in> tree2 \<Longrightarrow> (p2, c) \<in> tree2 \<Longrightarrow> p1 = p2\<close>
+  then show \<open>unique_parent tree2\<close>
   proof(cases \<open>move_time oper < log_time logop\<close>)
     case True
     moreover obtain tree1a where \<open>tree1a = undo_op (logop, tree1)\<close>
       by simp
-    moreover from this have 1: \<open>\<And>p1 p2 c. (p1, c) \<in> tree1a \<Longrightarrow> (p2, c) \<in> tree1a \<Longrightarrow> p1 = p2\<close>
-      using undo_op_unique_parent by (metis step.prems(3) log_op.exhaust_sel)
+    moreover from this have 1: \<open>unique_parent tree1a\<close>
+      using undo_op_unique_parent by (metis step.prems(1) log_op.exhaust_sel)
     moreover obtain ops1b tree1b where \<open>(ops1b, tree1b) = interp_op oper (ops, tree1a)\<close>
       by (metis surj_pair)
-    moreover from this have \<open>\<And>p1 p2 c. (p1, c) \<in> tree1b \<Longrightarrow> (p2, c) \<in> tree1b \<Longrightarrow> p1 = p2\<close>
+    moreover from this have \<open>unique_parent tree1b\<close>
       using 1 by (metis step.hyps)
-    ultimately show \<open>\<And>p1 p2 c. (p1, c) \<in> tree2 \<Longrightarrow> (p2, c) \<in> tree2 \<Longrightarrow> p1 = p2\<close>
-      using redo_op_unique_parent by (metis interp_op.simps(2) step.prems(4))
+    ultimately show \<open>unique_parent tree2\<close>
+      using redo_op_unique_parent by (metis interp_op.simps(2) step.prems(2))
   next
     case False
     hence \<open>snd (do_op (oper, tree1)) = tree2\<close>
-      by (metis (mono_tags, lifting) interp_op.simps(2) prod.sel(2) split_beta step.prems(4))
-    then show \<open>\<And>p1 p2 c. (p1, c) \<in> tree2 \<Longrightarrow> (p2, c) \<in> tree2 \<Longrightarrow> p1 = p2\<close>
-      by (metis do_op_unique_parent operation.exhaust_sel prod.exhaust_sel step.prems(3))
+      by (metis (mono_tags, lifting) interp_op.simps(2) prod.sel(2) split_beta step.prems(2))
+    then show \<open>unique_parent tree2\<close>
+      by (metis do_op_unique_parent operation.exhaust_sel prod.exhaust_sel step.prems(1))
   qed
 qed
 
-corollary interp_ops_unique_parent:
+theorem interp_ops_unique_parent:
   assumes \<open>interp_ops ops = (log, tree)\<close>
-  shows \<open>\<And>p1 p2 c. (p1, c) \<in> tree \<Longrightarrow> (p2, c) \<in> tree \<Longrightarrow> p1 = p2\<close>
+  shows \<open>unique_parent tree\<close>
 using assms proof(induction ops arbitrary: log tree rule: List.rev_induct)
   case Nil
+  hence \<open>interp_ops [] = ([], {})\<close>
+    by (simp add: interp_ops_def)
+  hence \<open>tree = {}\<close>
+    by (metis Nil.prems snd_conv)
   then show ?case
-    by (metis empty_iff foldl_Nil fst_conv interp_ops_def swap_simp)
+    by (simp add: unique_parent_def)
 next
   case (snoc x xs)
   obtain log tree where interp_xs: \<open>interp_ops xs = (log, tree)\<close>
     by fastforce
   hence \<open>interp_ops (xs @ [x]) = interp_op x (log, tree)\<close>
     by (simp add: interp_ops_def)
-  moreover have \<open>\<And>p1 p2 c. (p1, c) \<in> tree \<Longrightarrow> (p2, c) \<in> tree \<Longrightarrow> p1 = p2\<close>
+  moreover have \<open>unique_parent tree\<close>
     by (simp add: interp_xs snoc.IH)
   ultimately show ?case
     by (metis interp_op_unique_parent snoc.prems)
@@ -199,7 +289,7 @@ section \<open>Preserving the invariant that the tree contains no cycles\<close>
 
 inductive_cases ancestor_indcases: \<open>ancestor \<T> m p\<close>
 
-definition cyclic :: \<open>('n \<times> 'n) set \<Rightarrow> bool\<close>
+definition cyclic :: \<open>('n \<times> 'm \<times> 'n) set \<Rightarrow> bool\<close>
   where \<open>cyclic \<T> \<longleftrightarrow> (\<exists>n. ancestor \<T> n n)\<close>
 
 lemma cyclicE [elim]:
@@ -224,9 +314,9 @@ lemma acyclic_subset:
   shows \<open>\<not> cyclic S\<close>
   using assms ancestor_superset_closed by (metis cyclic_def)
 
-inductive path :: \<open>('n \<times> 'n) set \<Rightarrow> 'n \<Rightarrow> 'n \<Rightarrow> ('n \<times> 'n) list \<Rightarrow> bool\<close> where
-  \<open>\<lbrakk>(b, e) \<in> T\<rbrakk> \<Longrightarrow> path T b e [(b, e)]\<close> |
-  \<open>\<lbrakk>path T b m xs; (m, e) \<notin> set xs; (m, e) \<in> T\<rbrakk> \<Longrightarrow> path T b e (xs @ [(m, e)])\<close>
+inductive path :: \<open>('n \<times> 'm \<times> 'n) set \<Rightarrow> 'n \<Rightarrow> 'n \<Rightarrow> ('n \<times> 'n) list \<Rightarrow> bool\<close> where
+  \<open>\<lbrakk>(b, x, e) \<in> T\<rbrakk> \<Longrightarrow> path T b e [(b, e)]\<close> |
+  \<open>\<lbrakk>path T b m xs; (m, e) \<notin> set xs; (m, x, e) \<in> T\<rbrakk> \<Longrightarrow> path T b e (xs @ [(m, e)])\<close>
 
 inductive_cases path_indcases: \<open>path T b e xs\<close>
 
@@ -291,23 +381,26 @@ using assms proof(induction rule: path.induct, force)
     case True
     then show ?thesis using step.hyps by force
   next
-    case False (* (p, c) \<in> set xs *)
+    case pc_xs: False (* (p, c) \<in> set xs *)
     then obtain ys zs where yszs: \<open>(ys = [] \<or> path T b p ys) \<and> (zs = [] \<or> path T c m zs) \<and>
         xs = ys @ [(p, c)] @ zs \<and> (p, c) \<notin> set ys \<and> (p, c) \<notin> set zs\<close>
       using step.IH step.prems by auto
+    have path_zs: \<open>path T c e (zs @ [(m, e)])\<close>
+      by (metis (no_types, lifting) Un_iff append_Cons last_path path.simps
+          self_append_conv2 set_append step.hyps(1) step.hyps(2) step.hyps(3) yszs)
     then show ?thesis
     proof(cases \<open>ys = []\<close>)
       case True
       hence \<open>\<exists>zsa. ([] = [] \<or> path T b p []) \<and> (zsa = [] \<or> path T c e zsa) \<and>
               (p, c) # zs @ [(m, e)] = [] @ (p, c) # zsa \<and> (p, c) \<notin> set [] \<and> (p, c) \<notin> set zsa\<close>
-        using path.intros singleton_path step.hyps yszs by fastforce
+        using pc_xs path_zs yszs by auto
       then show ?thesis
         using yszs by force
     next
       case False
       hence \<open>\<exists>zsa. (ys = [] \<or> path T b p ys) \<and> (zsa = [] \<or> path T c e zsa) \<and>
               ys @ (p, c) # zs @ [(m, e)] = ys @ (p, c) # zsa \<and> (p, c) \<notin> set ys \<and> (p, c) \<notin> set zsa\<close>
-        using last_path path.intros step.hyps yszs by fastforce
+        using path_zs pc_xs yszs by auto
       then show ?thesis
         using yszs by force
     qed
@@ -318,10 +411,10 @@ lemma anc_path:
   assumes \<open>ancestor T p c\<close>
   shows \<open>\<exists>xs. path T p c xs\<close>
 using assms proof(induction rule: ancestor.induct)
-  case (1 parent child tree)
+  case (1 parent meta child tree)
   then show ?case by (meson path.intros(1))
 next
-  case step: (2 parent child tree anc)
+  case step: (2 parent meta child tree anc)
   then obtain xs where xs: \<open>path tree anc parent xs\<close>
     by blast
   then show ?case
@@ -345,14 +438,9 @@ lemma anc_path_eq:
   shows \<open>ancestor T p c \<longleftrightarrow> (\<exists>xs. path T p c xs)\<close>
   by (meson anc_path path_anc)
 
-lemma path_subset:
-  assumes \<open>path T m n xs\<close>
-  shows \<open>set xs \<subseteq> T\<close>
-using assms by (induction rule: path.induct) auto
-
 lemma rem_edge_path:
   assumes \<open>path T m n xs\<close>
-    and \<open>T = insert (p, c) S\<close>
+    and \<open>T = insert (p, x, c) S\<close>
     and \<open>(p, c) \<notin> set xs\<close>
   shows \<open>path S m n xs\<close>
 using assms by (induction rule: path.induct, auto simp add: path.intros)
@@ -364,7 +452,7 @@ lemma ancestor_transitive:
 
 lemma cyclic_path_technical:
   assumes \<open>path T m m xs\<close>
-    and \<open>T = insert (p, c) S\<close>
+    and \<open>T = insert (p, x, c) S\<close>
     and \<open>\<forall>n. \<not> ancestor S n n\<close>
     and \<open>c \<noteq> p\<close>
   shows \<open>ancestor S c p\<close>
@@ -390,7 +478,7 @@ next
 qed
 
 lemma cyclic_ancestor:
-  assumes \<open>cyclic (S \<union> {(p, c)})\<close>
+  assumes \<open>cyclic (S \<union> {(p, x, c)})\<close>
     and \<open>\<not> (cyclic S)\<close> 
     and \<open>c \<noteq> p\<close>
   shows \<open>ancestor S c p\<close>
@@ -398,7 +486,7 @@ using assms anc_path cyclic_def cyclic_path_technical by fastforce
 
 lemma do_op_acyclic:
   assumes \<open>\<not> cyclic tree1\<close>
-    and \<open>do_op (Move t newp c, tree1) = (log_oper, tree2)\<close>
+    and \<open>do_op (Move t newp m c, tree1) = (log_oper, tree2)\<close>
   shows \<open>\<not> cyclic tree2\<close>
 proof(cases \<open>ancestor tree1 c newp \<or> c = newp\<close>)
   case True
@@ -406,19 +494,18 @@ proof(cases \<open>ancestor tree1 c newp \<or> c = newp\<close>)
     using assms by auto
 next
   case False
-  hence A: \<open>tree2 = {(p', c') \<in> tree1. c' \<noteq> c} \<union> {(newp, c)}\<close>
+  hence A: \<open>tree2 = {(p', m', c') \<in> tree1. c' \<noteq> c} \<union> {(newp, m, c)}\<close>
     using assms(2) by auto
-  moreover have \<open>{(p', c') \<in> tree1. c' \<noteq> c} \<subseteq> tree1\<close>
+  moreover have \<open>{(p', m', c') \<in> tree1. c' \<noteq> c} \<subseteq> tree1\<close>
     by blast
   moreover have \<open>\<not> (cyclic tree1)\<close>
     using assms and cyclic_def by auto
-  moreover have \<open>\<not> (cyclic {(p', c') \<in> tree1. c' \<noteq> c})\<close>
+  moreover have B: \<open>\<not> (cyclic {(p', m', c') \<in> tree1. c' \<noteq> c})\<close>
     using acyclic_subset calculation(2) calculation(3) by blast
   {
     assume \<open>cyclic tree2\<close>
-    have \<open>ancestor {(p', c') \<in> tree1. c' \<noteq> c} c newp\<close>
-      using cyclic_ancestor using False
-      using A \<open>\<not> cyclic {(p', c'). (p', c') \<in> tree1 \<and> c' \<noteq> c}\<close> \<open>cyclic tree2\<close> by force
+    have \<open>ancestor {(p', m', c') \<in> tree1. c' \<noteq> c} c newp\<close>
+      using cyclic_ancestor False A B \<open>cyclic tree2\<close> by force
     from this have \<open>False\<close>
       using False ancestor_superset_closed calculation(2) by fastforce
   }
@@ -446,28 +533,17 @@ qed
 section \<open>Commutativity of move operation\<close>
 
 lemma interp_ops_base [simp]:
-  shows \<open>interp_ops [Move t1 p1 c1, Move t2 p2 c2] =
-                    interp_op (Move t2 p2 c2) (interp_op (Move t1 p1 c1) ([], {}))\<close>
-  by(clarsimp simp add: interp_ops_def)
-
-lemma interp_ops_base_commute:
-  assumes \<open>t1 \<noteq> t2\<close>
-  shows \<open>interp_ops [Move t1 p1 c1, Move t2 p2 c2] = interp_ops [Move t2 p2 c2, Move t1 p1 c1]\<close>
-  using assms by(cases \<open>t2 < t1\<close>; cases \<open>p1 = c1\<close>; cases \<open>p2 = c2\<close>; cases \<open>c1 = c2\<close>; force)
+  shows \<open>interp_ops [Move t1 p1 m1 c1, Move t2 p2 m2 c2] =
+                    interp_op (Move t2 p2 m2 c2) (interp_op (Move t1 p1 m1 c1) ([], {}))\<close>
+  by (clarsimp simp add: interp_ops_def)
 
 lemma interp_ops_step [simp]:
-  shows \<open>interp_ops (xs @ [x]) =
-                    interp_op x (interp_ops xs)\<close>
-  by(clarsimp simp add: interp_ops_def)
-
-lemma interp_ops_step_commute [simp]:
-  shows \<open>interp_ops (ops @ [Move t1 p1 c1, Move t2 p2 c2]) =
-          interp_op (Move t2 p2 c2) (interp_op (Move t1 p1 c1) (interp_ops ops))\<close>
-  by(clarsimp simp add: interp_ops_def)
+  shows \<open>interp_ops (xs @ [x]) = interp_op x (interp_ops xs)\<close>
+  by (clarsimp simp add: interp_ops_def)
 
 lemma interp_ops_Nil [simp]:
   shows \<open>interp_ops [] = ([], {})\<close>
-  by(clarsimp simp add: interp_ops_def)
+  by (clarsimp simp add: interp_ops_def)
 
 lemma distinct_list_pick1:
   assumes \<open>set (xs @ [x]) = set (ys @ [x] @ zs)\<close>
@@ -477,60 +553,63 @@ using assms by (induction xs) (fastforce+)
 
 lemma interp_op_commute_base:
   assumes \<open>t1 < t2\<close>
-    and \<open>\<And>p1 p2 c. (p1, c) \<in> tree \<Longrightarrow> (p2, c) \<in> tree \<Longrightarrow> p1 = p2\<close>
-  shows \<open>interp_op (Move t2 p2 c2) (interp_op (Move t1 p1 c1) ([], tree)) =
-         interp_op (Move t1 p1 c1) (interp_op (Move t2 p2 c2) ([], tree))\<close>
+    and \<open>unique_parent tree\<close>
+  shows \<open>interp_op (Move t2 p2 m2 c2) (interp_op (Move t1 p1 m1 c1) ([], tree)) =
+         interp_op (Move t1 p1 m1 c1) (interp_op (Move t2 p2 m2 c2) ([], tree))\<close>
 proof -
-  obtain tree1 where tree1: \<open>do_op (Move t1 p1 c1, tree) = (LogMove t1 (get_parent tree c1) p1 c1, tree1)\<close>
+  obtain tree1 where tree1: \<open>do_op (Move t1 p1 m1 c1, tree) =
+      (LogMove t1 (get_parent tree c1) p1 m1 c1, tree1)\<close>
     by simp
-  obtain tree12 where tree12: \<open>do_op (Move t2 p2 c2, tree1) = (LogMove t2 (get_parent tree1 c2) p2 c2, tree12)\<close>
+  obtain tree12 where tree12: \<open>do_op (Move t2 p2 m2 c2, tree1) =
+      (LogMove t2 (get_parent tree1 c2) p2 m2 c2, tree12)\<close>
     by simp
-  obtain tree2 where tree2: \<open>do_op (Move t2 p2 c2, tree) = (LogMove t2 (get_parent tree c2) p2 c2, tree2)\<close>
+  obtain tree2 where tree2: \<open>do_op (Move t2 p2 m2 c2, tree) =
+      (LogMove t2 (get_parent tree c2) p2 m2 c2, tree2)\<close>
     by simp
-  hence undo2: \<open>undo_op (LogMove t2 (get_parent tree c2) p2 c2, tree2) = tree\<close>
-    using assms(2) do_undo_op_inv by metis
+  hence undo2: \<open>undo_op (LogMove t2 (get_parent tree c2) p2 m2 c2, tree2) = tree\<close>
+    using assms(2) do_undo_op_inv by fastforce
   have \<open>\<not> t2 < t1\<close>
     using not_less_iff_gr_or_eq assms(1) by blast
-  hence \<open>interp_op (Move t2 p2 c2) (interp_op (Move t1 p1 c1) ([], tree)) =
-        ([LogMove t2 (get_parent tree1 c2) p2 c2, LogMove t1 (get_parent tree c1) p1 c1], tree12)\<close>
+  hence \<open>interp_op (Move t2 p2 m2 c2) (interp_op (Move t1 p1 m1 c1) ([], tree)) =
+        ([LogMove t2 (get_parent tree1 c2) p2 m2 c2, LogMove t1 (get_parent tree c1) p1 m1 c1], tree12)\<close>
     using tree1 tree12 by auto
-  moreover have \<open>interp_op (Move t2 p2 c2) ([], tree) = ([LogMove t2 (get_parent tree c2) p2 c2], tree2)\<close>
+  moreover have \<open>interp_op (Move t2 p2 m2 c2) ([], tree) =
+      ([LogMove t2 (get_parent tree c2) p2 m2 c2], tree2)\<close>
     using tree2 by auto
-  hence \<open>interp_op (Move t1 p1 c1) (interp_op (Move t2 p2 c2) ([], tree)) =
-         redo_op (LogMove t2 (get_parent tree c2) p2 c2) ([LogMove t1 (get_parent tree c1) p1 c1], tree1)\<close>
+  hence \<open>interp_op (Move t1 p1 m1 c1) (interp_op (Move t2 p2 m2 c2) ([], tree)) =
+         redo_op (LogMove t2 (get_parent tree c2) p2 m2 c2) ([LogMove t1 (get_parent tree c1) p1 m1 c1], tree1)\<close>
     using tree1 undo2 assms(1) by auto
   ultimately show ?thesis
     using tree12 by auto
 qed
 
 lemma interp_op_log_cons:
-  assumes \<open>interp_op (Move t1 p1 c1) (log, tree) = (log2, tree2)\<close>
+  assumes \<open>interp_op (Move t1 p1 m1 c1) (log, tree) = (log2, tree2)\<close>
   shows \<open>\<exists>logop rest. log2 = logop # rest \<and> t1 \<le> log_time logop\<close>
 proof(cases log)
   case Nil
   then show ?thesis using assms by auto
 next
   case (Cons logop rest)
-  obtain t2 oldp2 p2 c2 where logop: \<open>logop = LogMove t2 oldp2 p2 c2\<close>
+  obtain t2 oldp2 p2 m2 c2 where logop: \<open>logop = LogMove t2 oldp2 p2 m2 c2\<close>
     using log_op.exhaust by blast
   then show ?thesis
   proof(cases \<open>t1 < t2\<close>)
     case True
-    obtain tree1 log1 where tree1: \<open>interp_op (Move t1 p1 c1) (rest, undo_op (logop, tree)) = (log1, tree1)\<close>
+    obtain tree1 log1 where tree1: \<open>interp_op (Move t1 p1 m1 c1) (rest, undo_op (logop, tree)) = (log1, tree1)\<close>
       by fastforce
-    obtain tree12 where \<open>do_op (Move t2 p2 c2, tree1) = (LogMove t2 (get_parent tree1 c2) p2 c2, tree12)\<close>
+    obtain tree12 where \<open>do_op (Move t2 p2 m2 c2, tree1) = (LogMove t2 (get_parent tree1 c2) p2 m2 c2, tree12)\<close>
       by simp
-    hence \<open>interp_op (Move t1 p1 c1) (log, tree) =
-           (LogMove t2 (get_parent tree1 c2) p2 c2 # log1, tree12)\<close>
+    hence \<open>interp_op (Move t1 p1 m1 c1) (log, tree) = (LogMove t2 (get_parent tree1 c2) p2 m2 c2 # log1, tree12)\<close>
       using True local.Cons tree1 logop by auto
     then show ?thesis
       using True assms by auto
   next
     case False
-    obtain tree1 where tree1: \<open>do_op (Move t1 p1 c1, tree) = (LogMove t1 (get_parent tree c1) p1 c1, tree1)\<close>
+    obtain tree1 where tree1: \<open>do_op (Move t1 p1 m1 c1, tree) = (LogMove t1 (get_parent tree c1) p1 m1 c1, tree1)\<close>
       by simp
-    hence \<open>interp_op (Move t1 p1 c1) (log, tree) =
-           (LogMove t1 (get_parent tree c1) p1 c1 # log, tree1)\<close>
+    hence \<open>interp_op (Move t1 p1 m1 c1) (log, tree) =
+           (LogMove t1 (get_parent tree c1) p1 m1 c1 # log, tree1)\<close>
       using False local.Cons logop by auto
     then show ?thesis
       using assms by auto
@@ -539,114 +618,114 @@ qed
 
 lemma interp_op_commute2:
   assumes \<open>t1 < t2\<close>
-    and \<open>\<And>p1 p2 c. (p1, c) \<in> tree \<Longrightarrow> (p2, c) \<in> tree \<Longrightarrow> p1 = p2\<close>
+    and \<open>unique_parent tree\<close>
     and \<open>distinct ((map log_time log) @ [t1, t2])\<close>
-  shows \<open>interp_op (Move t2 p2 c2) (interp_op (Move t1 p1 c1) (log, tree)) =
-         interp_op (Move t1 p1 c1) (interp_op (Move t2 p2 c2) (log, tree))\<close>
+  shows \<open>interp_op (Move t2 p2 m2 c2) (interp_op (Move t1 p1 m1 c1) (log, tree)) =
+         interp_op (Move t1 p1 m1 c1) (interp_op (Move t2 p2 m2 c2) (log, tree))\<close>
 using assms proof(induction log arbitrary: tree)
   case Nil
   then show ?case using interp_op_commute_base by metis
 next
   case (Cons logop log)
-  have parent0: \<open>\<And>p1 c p2. (p1, c) \<in> undo_op (logop, tree) \<Longrightarrow> (p2, c) \<in> undo_op (logop, tree) \<Longrightarrow> p1 = p2\<close>
+  have parent0: \<open>unique_parent (undo_op (logop, tree))\<close>
     by (metis Cons.prems(2) log_op.exhaust_sel undo_op_unique_parent)
-  obtain t3 oldp3 p3 c3 where logop: \<open>logop = LogMove t3 oldp3 p3 c3\<close>
+  obtain t3 oldp3 p3 m3 c3 where logop: \<open>logop = LogMove t3 oldp3 p3 m3 c3\<close>
     using log_op.exhaust by blast
   then consider (c1) \<open>t3 < t1\<close> | (c2) \<open>t1 < t3 \<and> t3 < t2\<close> | (c3) \<open>t2 < t3\<close>
     using Cons.prems(3) by force
   then show ?case
   proof(cases)
     case c1 (* t3 < t1 < t2 *)
-    obtain tree1 where tree1: \<open>do_op (Move t1 p1 c1, tree) = (LogMove t1 (get_parent tree c1) p1 c1, tree1)\<close>
+    obtain tree1 where tree1: \<open>do_op (Move t1 p1 m1 c1, tree) = (LogMove t1 (get_parent tree c1) p1 m1 c1, tree1)\<close>
       by simp
-    obtain tree12 where tree12: \<open>do_op (Move t2 p2 c2, tree1) = (LogMove t2 (get_parent tree1 c2) p2 c2, tree12)\<close>
+    obtain tree12 where tree12: \<open>do_op (Move t2 p2 m2 c2, tree1) = (LogMove t2 (get_parent tree1 c2) p2 m2 c2, tree12)\<close>
       by simp
-    obtain tree2 where tree2: \<open>do_op (Move t2 p2 c2, tree) = (LogMove t2 (get_parent tree c2) p2 c2, tree2)\<close>
+    obtain tree2 where tree2: \<open>do_op (Move t2 p2 m2 c2, tree) = (LogMove t2 (get_parent tree c2) p2 m2 c2, tree2)\<close>
       by simp
-    hence undo2: \<open>undo_op (LogMove t2 (get_parent tree c2) p2 c2, tree2) = tree\<close>
+    hence undo2: \<open>undo_op (LogMove t2 (get_parent tree c2) p2 m2 c2, tree2) = tree\<close>
       using Cons.prems(2) do_undo_op_inv by metis
     have \<open>\<not> t2 < t1\<close>
       using not_less_iff_gr_or_eq Cons.prems(1) by blast
-    hence \<open>interp_op (Move t2 p2 c2) (interp_op (Move t1 p1 c1) (logop # log, tree)) =
-           ([LogMove t2 (get_parent tree1 c2) p2 c2, LogMove t1 (get_parent tree c1) p1 c1, logop] @ log, tree12)\<close>
+    hence \<open>interp_op (Move t2 p2 m2 c2) (interp_op (Move t1 p1 m1 c1) (logop # log, tree)) =
+           ([LogMove t2 (get_parent tree1 c2) p2 m2 c2, LogMove t1 (get_parent tree c1) p1 m1 c1, logop] @ log, tree12)\<close>
       using tree1 tree12 logop c1 by auto
     moreover have \<open>t3 < t2\<close>
       using c1 Cons.prems(1) by auto
-    hence \<open>interp_op (Move t2 p2 c2) (logop # log, tree) = (LogMove t2 (get_parent tree c2) p2 c2 # logop # log, tree2)\<close>
+    hence \<open>interp_op (Move t2 p2 m2 c2) (logop # log, tree) = (LogMove t2 (get_parent tree c2) p2 m2 c2 # logop # log, tree2)\<close>
       using tree2 logop by auto
-    hence \<open>interp_op (Move t1 p1 c1) (interp_op (Move t2 p2 c2) (logop # log, tree)) =
-           redo_op (LogMove t2 (get_parent tree c2) p2 c2) (LogMove t1 (get_parent tree c1) p1 c1 # logop # log, tree1)\<close>
+    hence \<open>interp_op (Move t1 p1 m1 c1) (interp_op (Move t2 p2 m2 c2) (logop # log, tree)) =
+           redo_op (LogMove t2 (get_parent tree c2) p2 m2 c2) (LogMove t1 (get_parent tree c1) p1 m1 c1 # logop # log, tree1)\<close>
       using Cons.prems(1) c1 logop tree1 undo2 by auto
     ultimately show ?thesis
       using tree12 by auto
   next
     case c2 (* t1 < t3 < t2 *)
-    obtain tree1 log1 where tree1: \<open>interp_op (Move t1 p1 c1) (log, undo_op (logop, tree)) = (log1, tree1)\<close>
+    obtain tree1 log1 where tree1: \<open>interp_op (Move t1 p1 m1 c1) (log, undo_op (logop, tree)) = (log1, tree1)\<close>
       by fastforce
-    obtain tree13 where tree13: \<open>do_op (Move t3 p3 c3, tree1) = (LogMove t3 (get_parent tree1 c3) p3 c3, tree13)\<close>
+    obtain tree13 where tree13: \<open>do_op (Move t3 p3 m3 c3, tree1) = (LogMove t3 (get_parent tree1 c3) p3 m3 c3, tree13)\<close>
       by simp
-    obtain tree132 where tree132: \<open>do_op (Move t2 p2 c2, tree13) = (LogMove t2 (get_parent tree13 c2) p2 c2, tree132)\<close>
+    obtain tree132 where tree132: \<open>do_op (Move t2 p2 m2 c2, tree13) = (LogMove t2 (get_parent tree13 c2) p2 m2 c2, tree132)\<close>
       by simp
-    obtain tree2 where tree2: \<open>do_op (Move t2 p2 c2, tree) = (LogMove t2 (get_parent tree c2) p2 c2, tree2)\<close>
+    obtain tree2 where tree2: \<open>do_op (Move t2 p2 m2 c2, tree) = (LogMove t2 (get_parent tree c2) p2 m2 c2, tree2)\<close>
       by simp
-    hence undo2: \<open>undo_op (LogMove t2 (get_parent tree c2) p2 c2, tree2) = tree\<close>
+    hence undo2: \<open>undo_op (LogMove t2 (get_parent tree c2) p2 m2 c2, tree2) = tree\<close>
       by (metis Cons.prems(2) do_undo_op_inv)
-    have \<open>interp_op (Move t2 p2 c2) (interp_op (Move t1 p1 c1) (logop # log, tree)) =
-           (LogMove t2 (get_parent tree13 c2) p2 c2 # LogMove t3 (get_parent tree1 c3) p3 c3 # log1, tree132)\<close>
+    have \<open>interp_op (Move t2 p2 m2 c2) (interp_op (Move t1 p1 m1 c1) (logop # log, tree)) =
+           (LogMove t2 (get_parent tree13 c2) p2 m2 c2 # LogMove t3 (get_parent tree1 c3) p3 m3 c3 # log1, tree132)\<close>
       using c2 logop tree1 tree13 tree132 by auto
-    moreover have \<open>interp_op (Move t2 p2 c2) (logop # log, tree) =
-                   (LogMove t2 (get_parent tree c2) p2 c2 # logop # log, tree2)\<close>
+    moreover have \<open>interp_op (Move t2 p2 m2 c2) (logop # log, tree) =
+                   (LogMove t2 (get_parent tree c2) p2 m2 c2 # logop # log, tree2)\<close>
       using c2 logop tree2 by auto
-    hence \<open>interp_op (Move t1 p1 c1) (interp_op (Move t2 p2 c2) (logop # log, tree)) =
-           (LogMove t2 (get_parent tree13 c2) p2 c2 # LogMove t3 (get_parent tree1 c3) p3 c3 # log1, tree132)\<close>
+    hence \<open>interp_op (Move t1 p1 m1 c1) (interp_op (Move t2 p2 m2 c2) (logop # log, tree)) =
+           (LogMove t2 (get_parent tree13 c2) p2 m2 c2 # LogMove t3 (get_parent tree1 c3) p3 m3 c3 # log1, tree132)\<close>
       using assms(1) undo2 c2 logop tree1 tree13 tree132 by auto
     ultimately show ?thesis by simp
   next
     case c3 (* t1 < t2 < t3 *)
-    obtain tree1 log1 where tree1: \<open>interp_op (Move t1 p1 c1) (log, undo_op (logop, tree)) = (log1, tree1)\<close>
+    obtain tree1 log1 where tree1: \<open>interp_op (Move t1 p1 m1 c1) (log, undo_op (logop, tree)) = (log1, tree1)\<close>
       by fastforce
-    obtain tree13 where tree13: \<open>do_op (Move t3 p3 c3, tree1) = (LogMove t3 (get_parent tree1 c3) p3 c3, tree13)\<close>
+    obtain tree13 where tree13: \<open>do_op (Move t3 p3 m3 c3, tree1) = (LogMove t3 (get_parent tree1 c3) p3 m3 c3, tree13)\<close>
       by simp
-    hence undo13: \<open>undo_op (LogMove t3 (get_parent tree1 c3) p3 c3, tree13) = tree1\<close>
+    hence undo13: \<open>undo_op (LogMove t3 (get_parent tree1 c3) p3 m3 c3, tree13) = tree1\<close>
     proof -
-      have \<open>\<And>p1 p2 c. (p1, c) \<in> tree1 \<Longrightarrow> (p2, c) \<in> tree1 \<Longrightarrow> p1 = p2\<close>
+      have \<open>unique_parent tree1\<close>
         by (meson interp_op_unique_parent parent0 tree1)
       thus ?thesis
         using do_undo_op_inv tree13 by metis
     qed
-    obtain tree12 log12 where tree12: \<open>interp_op (Move t2 p2 c2) (log1, tree1) = (log12, tree12)\<close>
+    obtain tree12 log12 where tree12: \<open>interp_op (Move t2 p2 m2 c2) (log1, tree1) = (log12, tree12)\<close>
       by fastforce
-    obtain tree123 where tree123: \<open>do_op (Move t3 p3 c3, tree12) = (LogMove t3 (get_parent tree12 c3) p3 c3, tree123)\<close>
+    obtain tree123 where tree123: \<open>do_op (Move t3 p3 m3 c3, tree12) = (LogMove t3 (get_parent tree12 c3) p3 m3 c3, tree123)\<close>
       by simp
-    obtain tree2 log2 where tree2: \<open>interp_op (Move t2 p2 c2) (log, undo_op (logop, tree)) = (log2, tree2)\<close>
+    obtain tree2 log2 where tree2: \<open>interp_op (Move t2 p2 m2 c2) (log, undo_op (logop, tree)) = (log2, tree2)\<close>
       by fastforce
-    obtain tree21 log21 where tree21: \<open>interp_op (Move t1 p1 c1) (log2, tree2) = (log21, tree21)\<close>
+    obtain tree21 log21 where tree21: \<open>interp_op (Move t1 p1 m1 c1) (log2, tree2) = (log21, tree21)\<close>
       by fastforce
-    obtain tree213 where tree213: \<open>do_op (Move t3 p3 c3, tree21) = (LogMove t3 (get_parent tree21 c3) p3 c3, tree213)\<close>
+    obtain tree213 where tree213: \<open>do_op (Move t3 p3 m3 c3, tree21) = (LogMove t3 (get_parent tree21 c3) p3 m3 c3, tree213)\<close>
       by simp
-    obtain tree23 where tree23: \<open>do_op (Move t3 p3 c3, tree2) = (LogMove t3 (get_parent tree2 c3) p3 c3, tree23)\<close>
+    obtain tree23 where tree23: \<open>do_op (Move t3 p3 m3 c3, tree2) = (LogMove t3 (get_parent tree2 c3) p3 m3 c3, tree23)\<close>
       by simp
-    hence undo23: \<open>undo_op (LogMove t3 (get_parent tree2 c3) p3 c3, tree23) = tree2\<close>
+    hence undo23: \<open>undo_op (LogMove t3 (get_parent tree2 c3) p3 m3 c3, tree23) = tree2\<close>
     proof -
-      have \<open>\<And>p1 p2 c. (p1, c) \<in> tree2 \<Longrightarrow> (p2, c) \<in> tree2 \<Longrightarrow> p1 = p2\<close>
+      have \<open>unique_parent tree2\<close>
         by (meson interp_op_unique_parent parent0 tree2)
       thus ?thesis
         using do_undo_op_inv tree23 by metis
     qed
-    have \<open>interp_op (Move t1 p1 c1) (logop # log, tree) =
-           (LogMove t3 (get_parent tree1 c3) p3 c3 # log1, tree13)\<close>
+    have \<open>interp_op (Move t1 p1 m1 c1) (logop # log, tree) =
+           (LogMove t3 (get_parent tree1 c3) p3 m3 c3 # log1, tree13)\<close>
       using assms(1) c3 logop tree1 tree13 by auto
-    hence \<open>interp_op (Move t2 p2 c2) (interp_op (Move t1 p1 c1) (logop # log, tree)) =
-           (LogMove t3 (get_parent tree12 c3) p3 c3 # log12, tree123)\<close>
+    hence \<open>interp_op (Move t2 p2 m2 c2) (interp_op (Move t1 p1 m1 c1) (logop # log, tree)) =
+           (LogMove t3 (get_parent tree12 c3) p3 m3 c3 # log12, tree123)\<close>
       using c3 tree12 tree123 undo13 by auto
-    moreover have \<open>interp_op (Move t2 p2 c2) (logop # log, tree) =
-          (LogMove t3 (get_parent tree2 c3) p3 c3 # log2, tree23)\<close>
+    moreover have \<open>interp_op (Move t2 p2 m2 c2) (logop # log, tree) =
+          (LogMove t3 (get_parent tree2 c3) p3 m3 c3 # log2, tree23)\<close>
       using c3 logop tree2 tree23 by auto
-    hence \<open>interp_op (Move t1 p1 c1) (interp_op (Move t2 p2 c2) (logop # log, tree)) =
-           (LogMove t3 (get_parent tree21 c3) p3 c3 # log21, tree213)\<close>
+    hence \<open>interp_op (Move t1 p1 m1 c1) (interp_op (Move t2 p2 m2 c2) (logop # log, tree)) =
+           (LogMove t3 (get_parent tree21 c3) p3 m3 c3 # log21, tree213)\<close>
       using assms(1) c3 undo23 tree21 tree213 by auto
-    moreover have \<open>interp_op (Move t2 p2 c2) (interp_op (Move t1 p1 c1) (log, undo_op (logop, tree))) =
-                   interp_op (Move t1 p1 c1) (interp_op (Move t2 p2 c2) (log, undo_op (logop, tree)))\<close>
+    moreover have \<open>interp_op (Move t2 p2 m2 c2) (interp_op (Move t1 p1 m1 c1) (log, undo_op (logop, tree))) =
+                   interp_op (Move t1 p1 m1 c1) (interp_op (Move t2 p2 m2 c2) (log, undo_op (logop, tree)))\<close>
       using Cons.IH Cons.prems(3) assms(1) parent0 by auto
     ultimately show ?thesis
       using tree1 tree12 tree123 tree2 tree21 tree213 by auto
@@ -655,14 +734,14 @@ qed
 
 lemma interp_op_timestamp:
   assumes \<open>distinct ((map log_time log1) @ [t])\<close>
-    and \<open>interp_op (Move t p c) (log1, tree1) = (log2, tree2)\<close>
+    and \<open>interp_op (Move t p m c) (log1, tree1) = (log2, tree2)\<close>
   shows \<open>distinct (map log_time log2) \<and> set (map log_time log2) = {t} \<union> set (map log_time log1)\<close>
 using assms proof(induction log1 arbitrary: tree1 log2 tree2)
   case Nil
   then show ?case by auto
 next
   case (Cons logop log)
-  obtain log3 tree3 where log3: \<open>interp_op (Move t p c) (log, undo_op (logop, tree1)) = (log3, tree3)\<close>
+  obtain log3 tree3 where log3: \<open>interp_op (Move t p m c) (log, undo_op (logop, tree1)) = (log3, tree3)\<close>
     using prod.exhaust_sel by blast
   have \<open>distinct ((map log_time log) @ [t])\<close>
     using Cons.prems(1) by auto
@@ -671,25 +750,25 @@ next
   then show ?case
   proof(cases \<open>t < log_time logop\<close>)
     case recursive_case: True
-    obtain t2 oldp2 p2 c2 where logop: \<open>logop = LogMove t2 oldp2 p2 c2\<close>
+    obtain t2 oldp2 p2 m2 c2 where logop: \<open>logop = LogMove t2 oldp2 p2 m2 c2\<close>
       using log_op.exhaust by blast
-    obtain tree4 where \<open>do_op (Move t2 p2 c2, tree3) = (LogMove t2 (get_parent tree3 c2) p2 c2, tree4)\<close>
+    obtain tree4 where \<open>do_op (Move t2 p2 m2 c2, tree3) = (LogMove t2 (get_parent tree3 c2) p2 m2 c2, tree4)\<close>
       by simp
-    hence \<open>interp_op (Move t p c) (logop # log, tree1) =
-           (LogMove t2 (get_parent tree3 c2) p2 c2 # log3, tree4)\<close>
+    hence \<open>interp_op (Move t p m c) (logop # log, tree1) =
+           (LogMove t2 (get_parent tree3 c2) p2 m2 c2 # log3, tree4)\<close>
       using logop log3 recursive_case by auto
     moreover from this have \<open>set (map log_time log2) = {t} \<union> set (map log_time (logop # log))\<close>
       using Cons.prems(2) IH logop by fastforce
-    moreover have \<open>distinct (map log_time (LogMove t2 (get_parent tree3 c2) p2 c2 # log3))\<close>
+    moreover have \<open>distinct (map log_time (LogMove t2 (get_parent tree3 c2) p2 m2 c2 # log3))\<close>
       using Cons.prems(1) IH logop recursive_case by auto
     ultimately show ?thesis
       using Cons.prems(2) by auto
   next
     case cons_case: False
-    obtain tree4 where \<open>do_op (Move t p c, tree1) = (LogMove t (get_parent tree1 c) p c, tree4)\<close>
+    obtain tree4 where \<open>do_op (Move t p m c, tree1) = (LogMove t (get_parent tree1 c) p m c, tree4)\<close>
       by simp
-    hence \<open>interp_op (Move t p c) (logop # log, tree1) =
-           (LogMove t (get_parent tree1 c) p c # logop # log, tree4)\<close>
+    hence \<open>interp_op (Move t p m c) (logop # log, tree1) =
+           (LogMove t (get_parent tree1 c) p m c # logop # log, tree4)\<close>
       by (simp add: cons_case)
     moreover from this have \<open>set (map log_time log2) = {t} \<union> set (map log_time (logop # log))\<close>
       using Cons.prems(2) by auto
@@ -720,19 +799,19 @@ qed
 
 lemma interp_op_commute_last:
   assumes \<open>distinct ((map move_time ops) @ [t1, t2])\<close>
-  shows \<open>interp_ops (ops @ [Move t1 p1 c1, Move t2 p2 c2]) =
-         interp_ops (ops @ [Move t2 p2 c2, Move t1 p1 c1])\<close>
+  shows \<open>interp_ops (ops @ [Move t1 p1 m1 c1, Move t2 p2 m2 c2]) =
+         interp_ops (ops @ [Move t2 p2 m2 c2, Move t1 p1 m1 c1])\<close>
 proof -
   obtain log tree where interp_ops: \<open>interp_ops ops = (log, tree)\<close>
     by fastforce
-  hence unique_parent: \<open>\<And>p1 p2 c. (p1, c) \<in> tree \<Longrightarrow> (p2, c) \<in> tree \<Longrightarrow> p1 = p2\<close>
+  hence unique_parent: \<open>unique_parent tree\<close>
     by (meson interp_ops_unique_parent)
   have distinct_times: \<open>distinct ((map log_time log) @ [t1, t2])\<close>
     using assms interp_ops interp_ops_timestamps by auto
-  have \<open>interp_ops (ops @ [Move t1 p1 c1, Move t2 p2 c2]) =
-        interp_op (Move t2 p2 c2) (interp_op (Move t1 p1 c1) (log, tree))\<close>
-    using interp_ops by simp
-  also have \<open>... = interp_op (Move t1 p1 c1) (interp_op (Move t2 p2 c2) (log, tree))\<close>
+  have \<open>interp_ops (ops @ [Move t1 p1 m1 c1, Move t2 p2 m2 c2]) =
+        interp_op (Move t2 p2 m2 c2) (interp_op (Move t1 p1 m1 c1) (log, tree))\<close>
+    using interp_ops by (simp add: interp_ops_def)
+  also have \<open>... = interp_op (Move t1 p1 m1 c1) (interp_op (Move t2 p2 m2 c2) (log, tree))\<close>
   proof(cases \<open>t1 < t2\<close>)
     case True
     then show ?thesis
@@ -746,8 +825,8 @@ proof -
     ultimately show ?thesis
       by (metis unique_parent interp_op_commute2)
   qed
-  also have \<open>... = interp_ops (ops @ [Move t2 p2 c2, Move t1 p1 c1])\<close>
-    using interp_ops by simp
+  also have \<open>... = interp_ops (ops @ [Move t2 p2 m2 c2, Move t1 p1 m1 c1])\<close>
+    using interp_ops by (simp add: interp_ops_def)
   ultimately show ?thesis
     by presburger
 qed
